backend/Mach.v
@@ -448,13 +448,11 @@ Inductive callstack_function_defined : list stackframe -> Prop :=
       callstack_function_defined (Stackframe fb sp' ra c' :: cs').
 
 Inductive list_prefix : list (option (block * frame_info)) -> stack_adt -> Prop :=
-| list_prefix_nil s: list_prefix nil s
+| list_prefix_nil s: (forall b o, init_sp = Vptr b o -> in_stack s b) -> list_prefix nil s
 | list_prefix_cons lsp s f r sp bi
                        (REC: list_prefix lsp s)
-                       (BLOCKS: frame_adt_blocks f = (sp,bi)::nil)
-                       (NOINIT: forall b o, init_sp = Vptr b o -> ~ in_frames (f::r) b):
+                       (BLOCKS: frame_adt_blocks f = (sp,bi)::nil):
     list_prefix (Some (sp,bi) :: lsp) ( (f :: r) :: s).
-
 
 Definition stack_blocks_of_callstack (l : list stackframe) : list (option (block * frame_info)) :=
   map (fun x =>
@@ -476,13 +474,11 @@ Inductive call_stack_consistency: state -> Prop :=
       call_stack_consistency (State cs' fb (Vptr sp' Ptrofs.zero) c rs m')
 | call_stack_consistency_call:
     forall cs' fb rs m'
-      (NOINITHD: forall b o, init_sp = Vptr b o -> ~ in_frames (hd nil (Mem.stack_adt m')) b)
       (CallStackConsistency: list_prefix (stack_blocks_of_callstack cs') (tl (Mem.stack_adt m')))
       (CFD: callstack_function_defined cs'),
       call_stack_consistency (Callstate cs' fb rs m')
 | call_stack_consistency_return:
     forall cs' rs m'
-      (NOINITHD: forall b o, init_sp = Vptr b o -> ~ in_frames (hd nil (Mem.stack_adt m')) b)
       (CallStackConsistency: list_prefix (stack_blocks_of_callstack cs') (tl (Mem.stack_adt m')))
       (CFD: callstack_function_defined cs'),
       call_stack_consistency (Returnstate cs' rs m').
@@ -508,30 +504,24 @@ Proof.
   destruct 1; simpl; intros SIZECORRECT CSC; inv CSC; try now (econstructor; eauto).
   - econstructor; eauto. erewrite store_stack_no_abstract; eauto.
   - econstructor; eauto. destruct a; simpl in *; try discriminate. erewrite Mem.store_no_abstract; eauto.
-  - econstructor. rewrite_stack_blocks. simpl. easy. simpl in *. 
+  - econstructor. rewrite_stack_blocks. simpl. 
     rewrite FIND. repeat rewrite_stack_blocks. simpl. auto.
     econstructor; eauto.
   - econstructor; repeat rewrite_stack_blocks. auto.
     inv CallStackConsistency; simpl; auto.
-    inv CallStackConsistency; simpl; auto. auto.
+    inv CallStackConsistency; simpl; auto.
   - econstructor; eauto. repeat rewrite_stack_blocks; simpl; eauto.
   - econstructor; eauto; repeat rewrite_stack_blocks; simpl; eauto.
-    inv CallStackConsistency. eauto.    inv CallStackConsistency. eauto.
-  - econstructor; eauto. repeat rewrite_stack_blocks; simpl; eauto.
+    inv CallStackConsistency. eauto.
+  - econstructor; eauto; repeat rewrite_stack_blocks; simpl; eauto.
+    repeat econstructor; eauto.
     rewrite store_stack_no_abstract in EQ1 by eauto.
     revert EQ1; rewrite_stack_blocks. intro. rewrite EQ1 in CallStackConsistency. simpl in *.
-    constructor; auto. rewrite EQ1 in NOINITHD. simpl in NOINITHD.
-    intros. rewrite in_frames_cons. intros [A|A].
-    destruct A as [A|[]]. simpl in A; subst.
-    
-    intros.
-  - econstructor; eauto. repeat rewrite_stack_blocks; simpl; eauto.
-  - inv CFD. econstructor; eauto. repeat rewrite_stack_blocks; simpl; eauto.
-    rewrite EQ in *; simpl in *.
-    rewrite FINDF in CallStackConsistency.
-    inv CallStackConsistency. constructor; auto.
+    auto.
+  - econstructor; eauto; repeat rewrite_stack_blocks; simpl; eauto.
+  - inv CFD. econstructor; eauto; repeat rewrite_stack_blocks; simpl; eauto.
+    simpl in *; eauto. rewrite FINDF in CallStackConsistency. eauto.
 Qed.
-
 
 Inductive callstack_not_init : list stackframe -> Prop :=
 | cni_empty:
@@ -626,6 +616,18 @@ Ltac rewnb :=
       eapply Ple_trans; [ | apply external_call_nextblock in H; exact H ]
     end.
 
+Opaque Z.mul Z.add.
+
+Lemma lp_has_init_sp s m:
+  list_prefix s m ->
+  forall b o,
+    init_sp = Vptr b o ->
+    in_stack m b.
+Proof.
+  induction 1; simpl; intros; eauto.
+  rewrite in_stack_cons. right; eauto.    
+Qed.
+
 Theorem np_step:
   forall s1 t s2,
     step s1 t s2 ->
@@ -639,117 +641,57 @@ Proof.
       try (destr;[idtac]); repeat rewrite_stack_blocks;
         rewnb; eauto;
           try assumption.
-
-  destruct MSISHS as (fi & INS & O).
-  exists fi; split; eauto. destruct INS as (ff & fr & A & B & C).
-  exists ff, fr; repeat split; eauto. right; auto.
-  constructor; auto.
-  xomega.
-  revert EQ1; repeat rewrite_stack_blocks. intro.
-  unfold is_stack_top. simpl. intros [A|A].
-  subst b.
-  eapply Mem.fresh_block_alloc in ISP'VALID; eauto.
-  
-  exploit Mem.in_frames_valid. rewrite EQ1. rewrite in_stack_cons; left. unfold in_frames. unfold get_frames_blocks. apply A.
-  eapply Mem.fresh_block_alloc; eauto.
-
-  
-  rewrite_stack_blocks. assumption.
-  
-  Ltac rewtac :=
-     repeat match goal with
-             | H: Mem.nextblock ?m = _ |- Mem.valid_block ?m ?b => red; rewrite H; eauto
-             | H: Ple (Mem.nextblock ?m) (Mem.nextblock ?m'),
-                  H': Mem.valid_block ?m ?b |- Mem.valid_block ?m' ?b => unfold Mem.valid_block in *; xomega
-             | H: Mem.nextblock ?m = _ |- context [Mem.nextblock ?m] => rewrite H; eauto
-             (* | H: Mem.stack_adt ?m = _ |- ~ is_stack_top (Mem.stack_adt ?m) ?b => *)
-             (*   rewrite H; eauto *)
-             | H: Mem.stack_adt ?m = _ |- context [ (Mem.stack_adt ?m) ] =>
-               rewrite H; eauto
-             (* | H: Mem.stack_adt ?m = _ |- context [get_frame_info (Mem.stack_adt ?m) ?b] => *)
-             (*   rewrite H; eauto *)
-             | |- match init_sp with _ => _ end => (destruct init_sp eqn:?; auto); [idtac]
-             | |- init_sp_has_stackinfo ?m => unfold init_sp_has_stackinfo in *; destruct init_sp; auto 
-             end.
-  destruct 1; simpl; intros CSC NPM; inv NPM; constructor; intros; eauto;
-    repeat match goal with
-           | H: store_stack _ _ _ _ _ = Some _ |- _ =>
-             generalize (store_stack_no_abstract _ _ _ _ _ _ H);
-               generalize (store_stack_nextblock _ _ _ _ _ _ H);
-               revert H
-           | H: Mem.storev _ _ ?a _ = Some _ |- _ =>
-             destruct a; simpl in H; try discriminate;
-               generalize (Mem.store_no_abstract _ _ _ _ _ _ H);
-               generalize (Mem.nextblock_store _ _ _ _ _ _ H);
-               revert H
-           | H: Mem.free _ _ _ _ = Some _ |- _ =>
-             generalize (Mem.nextblock_free _ _ _ _ _ H);
-               generalize (Mem.free_no_abstract _ _ _ _ _ H);
-               revert H
-           | H: Mem.alloc _ _ _ = _ |- _ =>
-             generalize (Mem.nextblock_alloc _ _ _ _ _ H);
-               generalize (Mem.alloc_no_abstract _ _ _ _ _ H);
-               revert H
-           | H: Mem.unrecord_stack_block _ = Some _ |- _ =>
-             generalize (Mem.unrecord_stack_block_mem_unchanged _ _ H);
-               let A := fresh in
-               intro A; decompose [and] A; clear A;
-                 generalize (fun b => Mem.unrecord_stack_block_get_frame_info _ _ b H);
-                 revert H
-           | H: Mem.record_stack_blocks _ _ = Some _ |- _ =>
-             generalize (Mem.record_stack_blocks_mem_unchanged _ _ _ H);
-               let A := fresh in
-               intro A; decompose [and] A; clear A;
-               generalize (Mem.record_stack_blocks_stack_adt _ _ _ H);
-               revert H
-           | |- context [ Mem.nextblock (Mem.push_new_stage ?m)] => rewrite Mem.push_new_stage_nextblock
-           | |- Mem.valid_block (Mem.push_new_stage _) _ => red; rewrite Mem.push_new_stage_nextblock
-           | H: external_call _ _ _ _ _ _ _ |- _ =>
-             generalize (external_call_nextblock _ _ _ _ _ _ _ H);
-               generalize (eq_sym (external_call_stack_blocks _ _ _ _ _ _ _ H));
-               revert H
-           end. ; intros;
-      eauto;
-        unfold block_prop in *;
-     rewtac.
+  - destruct MSISHS as (fi & INS & O).
+    exists fi; split; eauto. destruct INS as (ff & fr & A & B & C).
+    exists ff, fr; repeat split; eauto. right; auto.
   - constructor; auto.
-  - edestruct Mem.unrecord_stack_adt; eauto. rewrite <- H9, H11 in MSISHS.
-    destruct MSISHS as (fr & fi & INFR & INS & RNGpriv & ARGS).
-    exists fr, fi; split; eauto.
-    split; eauto.
-    simpl in INS. destruct INS; auto.
-    rewrite <- H9, H11 in ISP'NST. subst. exfalso; apply ISP'NST.
-    red; simpl.
-    eapply in_frame_blocks_in_frame in INFR. red in INFR. auto.
   - xomega.
-  - edestruct Mem.unrecord_stack_adt; eauto. rewrite <- H8, H10 in *.
-    destruct MSISHS as (fr & fi & INFR & INS & RNGpriv & ARGS).
-    exists fr, fi; split; eauto.
-    split; eauto.
-    simpl in INS. destruct INS; auto.
-    subst. exfalso; apply ISP'NST.
-    red; simpl. eapply in_frame_blocks_in_frame; eauto.
-  - red in ISP'VALID. xomega.
-  - unfold is_stack_top.
-    simpl. intuition. subst b.
+  - revert EQ1; repeat rewrite_stack_blocks. intro.
+    unfold is_stack_top. simpl. intros [A|A].
+    subst b.
+    eapply Mem.fresh_block_alloc in ISP'VALID; eauto.
+    revert Heqv. inv CSC. 
+    intros.
+    eapply lp_has_init_sp in CallStackConsistency; eauto.
+    rewrite EQ1 in CallStackConsistency. simpl in CallStackConsistency.
+    exploit Mem.stack_norepet. intro ND. rewrite EQ1 in ND. revert Heqv. inv ND.
+    eapply H7 in CallStackConsistency; eauto.
+  - revert EQ1; repeat rewrite_stack_blocks. intro.
+    rewrite EQ1 in MSISHS.
+    destruct MSISHS as (fi & INS & O).
+    exists fi; split; eauto. destruct INS as (ff & fr & A & B & C).
+    destruct C. subst f0.
+    eexists ff, (_ :: fr); repeat split; eauto. right; auto. left; reflexivity.
+    exists ff, fr; repeat split; eauto. right; auto.
+  - xomega.
+  - intros; subst. intro; subst stk.
     eapply Mem.fresh_block_alloc; eauto.
-  - edestruct Mem.record_stack_blocks_stack_adt; eauto. 
-    destruct MSISHS as (fr & fi & INFR & INS & RNGpriv & ARGS).
-    exists fr, fi; split; eauto.
-    split; eauto. simpl; auto.
-  - xomega.
-  - intros. intro. subst.
-    eapply Mem.fresh_block_alloc; eauto.
-  - xomega.
-  - clearbody step. revert Heqv; inv CSC; inv NI.
-    destruct CallStackConsistency as (l1 & l2 & A & B). inv B.
-    unfold is_stack_top, get_stack_top_blocks.
-    inv CFD. rewrite FINDF in H1. destruct b1. simpl in *. subst.
-    destruct (Mem.stack_adt m) eqn:S. simpl; easy. 
-    inv A. simpl. intuition.
-    subst. edestruct NI0; eauto. 
-  - inv NI. auto.
-  - inv NI. auto.
+  - rewrite EQ. simpl. revert Heqv. inv CSC.
+    rewrite EQ in CallStackConsistency. simpl in CallStackConsistency.
+    inv CFD. rewrite FINDF in CallStackConsistency. inv CallStackConsistency.
+    intros Heqv.
+    eapply lp_has_init_sp in REC; eauto.
+    unfold is_stack_top. simpl.
+    exploit Mem.stack_norepet. intro ND. rewrite <- H4 in ND. revert Heqv. inv ND.
+    intros. intro INFR.
+    eapply H3 in REC; eauto.
+  - destruct MSISHS as (fi & INS & O).
+    exists fi; split; eauto. destruct INS as (ff & fr & A & B & C).
+    rewrite EQ in C |- *. simpl.
+    destruct C; eauto.
+    2: eexists; eauto.
+    exfalso. subst f0.
+    revert Heqv. inv CSC. intro.
+    eapply lp_has_init_sp in CallStackConsistency; eauto. rewrite EQ in CallStackConsistency; simpl in CallStackConsistency.
+    exploit Mem.stack_norepet. intro ND. rewrite EQ in ND. revert Heqv. inv ND.
+    intros. 
+    eapply H3 in CallStackConsistency; eauto.
+    eapply in_frame_in_frames; eauto.
+    red. unfold get_frame_blocks.
+    change b with (fst (b, fi)); apply in_map; eauto.
+  - intros; intro; subst. inv NI.
+    eapply NI0; eauto.
+  - inv NI; auto.
 Qed.
 
 
